Checkpoint pb proof

src/program_proof/simplepb/pb_definitions.v
@@ -1,19 +1,37 @@
 From Perennial.program_proof Require Import grove_prelude.
 From Goose.github_com.mit_pdos.gokv.simplepb Require Import pb.
 From Perennial.program_proof.grove_shared Require Import urpc_proof urpc_spec.
+From iris.base_logic Require Export lib.ghost_var.
+From iris.base_logic Require Export mono_nat.
 
 Section pb_definitions.
 
 Context `{!heapGS Σ}.
 
-Record pb_system_names :=
+Record pb_server_names :=
 {
-
+  urpc_gn: server_chan_gnames ;
+  epoch_gn: gname ;
 }.
 
-Implicit Type γ : pb_system_names.
+Implicit Type γ : pb_server_names.
 
 Implicit Type σ : list (list u8).
+
+Definition proposal_ptsto γ (epoch:u64) (σ:list (list u8)) : iProp Σ.
+Admitted.
+
+Definition accepted_lb γ (epoch:u64) (σ:list (list u8)) : iProp Σ.
+Admitted.
+
+Context `{!mono_natG Σ}.
+
+Definition own_epoch γ (epoch:u64) : iProp Σ :=
+  mono_nat_auth_own γ.(epoch_gn) 1 (int.nat epoch).
+
+Definition is_epoch_lb γ (epoch:u64) : iProp Σ :=
+  mono_nat_lb_own γ.(epoch_gn) (int.nat epoch).
+
 
 Definition own_Server (s:loc) γ : iProp Σ :=
   ∃ (epoch:u64) (nextIndex:u64) (isPrimary:bool) (sm:loc) (clerks:Slice.t),
@@ -25,6 +43,7 @@ Definition own_Server (s:loc) γ : iProp Σ :=
   "Hclerks" ∷ s ↦[pb.Server :: "clerks"] (slice_val clerks) ∗
 
   (* ghost *)
+  "HepochGhost" ∷ own_epoch γ epoch ∗
 
   (* durable *)
 
@@ -52,23 +71,48 @@ Admitted.
 Definition has_encoding_Error (encoded:list u8) (error:u64) : Prop.
 Admitted.
 
-Definition proposal_ptsto (epoch:u64) (σ:list (list u8)) : iProp Σ.
-Admitted.
-
-Definition accepted_lb (epoch:u64) (σ:list (list u8)) : iProp Σ.
-Admitted.
-
-Definition ApplyAsBackup_spec (encoded_args:list u8) Φ : iProp Σ :=
-  ∃ args σ,
+Program Definition ApplyAsBackup_spec γ :=
+  λ (encoded_args:list u8), λne (Φ : list u8 -d> iPropO Σ) ,
+  (∃ args σ,
     ⌜has_encoding_ApplyArgs encoded_args args⌝ ∗
     ⌜length σ = int.nat args.(index)⌝ ∗
     ⌜last σ = Some args.(op)⌝ ∗
-    proposal_ptsto args.(epoch) σ ∗
+    proposal_ptsto γ args.(epoch) σ ∗
     (∀ error (reply:list u8),
         ⌜has_encoding_Error reply error⌝ -∗
-        (if (decide (error = 0)) then accepted_lb args.(epoch) σ else True) -∗
+        (if (decide (error = 0)) then accepted_lb γ args.(epoch) σ else True) -∗
         Φ reply)
+    )%I
 .
+Next Obligation.
+  solve_proper.
+Defined.
+
+Context `{!urpcregG Σ}.
+
+Definition is_pb_host γ (host:chan) :=
+  handler_spec γ.(urpc_gn) host (U64 0) (ApplyAsBackup_spec γ).
+
+Definition is_Clerk (ck:loc) γ : iProp Σ :=
+  ∃ (cl:loc) srv,
+  "#Hcl" ∷ readonly (ck ↦[pb.Clerk :: "cl"] #cl) ∗
+  "#Hcl_rpc"  ∷ is_uRPCClient cl srv ∗
+  "#Hsrv" ∷ is_pb_host γ srv
+.
+
+Lemma wp_Server__epochFence (s:loc) γ (currEpoch epoch:u64) :
+  {{{
+        is_epoch_lb γ epoch ∗
+        s ↦[pb.Server :: "epoch"] #currEpoch ∗
+        own_epoch γ currEpoch
+  }}}
+    pb.Server__epochFence #s #epoch
+  {{{
+        RET #(negb (bool_decide (int.nat currEpoch = int.nat epoch))); s ↦[pb.Server :: "epoch"] #currEpoch ∗ own_epoch γ currEpoch
+  }}}
+.
+Proof.
+Admitted.
 
 Lemma wp_Server__ApplyAsBackup (s:loc) (args_ptr:loc) γ (epoch index:u64) (op:list u8) op_sl :
   is_Server s γ -∗
@@ -76,12 +120,8 @@ Lemma wp_Server__ApplyAsBackup (s:loc) (args_ptr:loc) γ (epoch index:u64) (op:l
         "HargEpoch" ∷ args_ptr ↦[pb.ApplyArgs :: "epoch"] #epoch ∗
         "HargIndex" ∷ args_ptr ↦[pb.ApplyArgs :: "index"] #index ∗
         "HargOp" ∷ args_ptr ↦[pb.ApplyArgs :: "op"] (slice_val op_sl) ∗
-        "HopSl" ∷ is_slice op_sl byteT 1 op
-        (* TODO:
-           ∗ epoch lower bound
-           ∗ (epoch, index) ↦ blah
-           ∗
-         *)
+        "HopSl" ∷ is_slice op_sl byteT 1 op ∗
+        "#HepochLb" ∷ is_epoch_lb γ epoch
   }}}
     pb.Server__ApplyAsBackup #s #args_ptr
   {{{
@@ -99,7 +139,23 @@ Proof.
   iNamed "Hown".
   wp_pures.
   wp_loadField.
+  wp_apply (wp_Server__epochFence with "[$Hepoch $HepochGhost $HepochLb]").
+  iIntros "Hepoch".
+  wp_if_destruct.
+  { (* return error: stale *)
+    admit.
+  }
+  replace (epoch0) with (epoch) by word.
 
+  wp_loadField.
+  wp_loadField.
+  wp_if_destruct.
+  { (* return errror: out-of-order *)
+    admit.
+  }
+
+  wp_loadField.
+  wp_loadField.
 Admitted.
 
 Lemma wp_Server__Apply (s:loc) γ op_sl:
